Generalize proofs a little bit for and_inplace as well

providers/quic/Impl.QUIC.fst
@@ -333,16 +333,6 @@ let create_in i r dst initial_pn traffic_secret =
 
       Success
 
-val xor_inplace (dst src: B.buffer U8.t) (len: U32.t { B.length dst = U32.v len }):
-  Stack unit
-    (requires fun h0 ->
-      B.(all_live h0 [ buf dst; buf src ]) /\
-      B.disjoint dst src /\
-      B.length dst = B.length src)
-    (ensures fun h0 _ h1 ->
-      B.(modifies (loc_buffer dst) h0 h1) /\
-      B.as_seq h1 dst `S.equal` Spec.QUIC.xor_inplace (B.as_seq h0 dst) (B.as_seq h0 src) 0)
-
 let lemma_slice s (i: nat { i <= S.length s }): Lemma
   (ensures (s `S.equal` S.append (S.slice s 0 i) (S.slice s i (S.length s))))
 =
@@ -397,68 +387,55 @@ let rec pointwise_upd (#a: eqtype) f b1 b2 i pos (x: a): Lemma
     ) i x;
   (S.equal) { lemma_slice b1 (i + 1) }
     S.upd (Spec.QUIC.pointwise_op f b1 b2 pos) i x;
-  };
-  ()
+  }
 
 #push-options "--z3rlimit 50"
-let rec lemma_xor_inplace0 (s1 s2: S.seq U8.t) (i: nat): Lemma
+let rec pointwise_seq_map2 (#a: eqtype) (f: a -> a -> a) (s1 s2: S.seq a) (i: nat): Lemma
   (requires (
     let l = S.length s1 in
     S.length s2 = l - i /\ i <= S.length s1))
   (ensures (
     let l = S.length s1 in
-    Spec.Loops.seq_map2 U8.logxor (S.slice s1 i l) s2 `S.equal`
-    S.slice (Spec.QUIC.xor_inplace s1 s2 i) i l))
+    Spec.Loops.seq_map2 f (S.slice s1 i l) s2 `S.equal`
+    S.slice (Spec.QUIC.pointwise_op f s1 s2 i) i l))
   (decreases (S.length s2))
 =
   if S.length s2 = 0 then
     ()
   else
     let l = S.length s1 in
-    let s2l = S.slice s2 0 1 in
-    let s2r = S.slice s2 1 (S.length s2) in
-    let s1p = S.slice s1 0 i in
-    let s1l = S.slice s1 i (i + 1) in
-    let s1r = S.slice s1 (i + 1) l in
-    assert S.(s2 `equal` (s2l @| s2r));
-    assert S.(s1 `equal` (s1p @| s1l @| s1r));
-    assert (i < S.length s1);
-    assert (i < S.length (Spec.QUIC.xor_inplace s1 s2 i));
     calc (S.equal) {
-      Spec.Loops.seq_map2 U8.logxor (S.slice s1 i l) s2;
+      Spec.Loops.seq_map2 f (S.slice s1 i l) s2;
     (S.equal) {}
-      S.cons (U8.logxor (S.head (S.slice s1 i l)) (S.head s2))
-        (Spec.Loops.seq_map2 U8.logxor (S.tail (S.slice s1 i l)) (S.tail s2));
+      S.cons (f (S.head (S.slice s1 i l)) (S.head s2))
+        (Spec.Loops.seq_map2 f (S.tail (S.slice s1 i l)) (S.tail s2));
     (S.equal) {}
-      S.cons (U8.logxor (S.head (S.slice s1 i l)) (S.head s2))
-        (Spec.Loops.seq_map2 U8.logxor (S.slice s1 (i + 1) l) (S.tail s2));
-    (S.equal) { lemma_xor_inplace0 s1 (S.slice s2 1 (S.length s2)) (i + 1) }
-      S.cons (U8.logxor (S.head (S.slice s1 i l)) (S.head s2))
-        (S.slice (Spec.QUIC.xor_inplace s1 (S.tail s2) (i + 1)) (i + 1) l);
-    (S.equal) { }
-      S.cons (U8.logxor (S.head (S.slice s1 i l)) (S.head s2))
-        (S.slice (Spec.QUIC.pointwise_op U8.logxor s1 (S.tail s2) (i + 1)) (i + 1) l);
+      S.cons (f (S.head (S.slice s1 i l)) (S.head s2))
+        (Spec.Loops.seq_map2 f (S.slice s1 (i + 1) l) (S.tail s2));
+    (S.equal) { pointwise_seq_map2 f s1 (S.slice s2 1 (S.length s2)) (i + 1) }
+      S.cons (f (S.head (S.slice s1 i l)) (S.head s2))
+        (S.slice (Spec.QUIC.pointwise_op f s1 (S.tail s2) (i + 1)) (i + 1) l);
     (S.equal) { }
       S.slice (
-        S.upd (Spec.QUIC.pointwise_op U8.logxor s1 (S.tail s2) (i + 1))
+        S.upd (Spec.QUIC.pointwise_op f s1 (S.tail s2) (i + 1))
           i
-          (U8.logxor (S.head (S.slice s1 i l)) (S.head s2)))
+          (f (S.head (S.slice s1 i l)) (S.head s2)))
         i
         l;
     (S.equal) { }
       S.slice (
-        S.upd (Spec.QUIC.pointwise_op U8.logxor s1 (S.slice s2 1 (S.length s2)) (i + 1))
+        S.upd (Spec.QUIC.pointwise_op f s1 (S.slice s2 1 (S.length s2)) (i + 1))
           i
-          (U8.logxor (S.head (S.slice s1 i l)) (S.head s2)))
+          (f (S.head (S.slice s1 i l)) (S.head s2)))
         i
         l;
     (S.equal) {
-      pointwise_upd U8.logxor s1 (S.slice s2 1 (S.length s2)) i (i + 1)
-        (U8.logxor (S.head (S.slice s1 i l)) (S.head s2))
+      pointwise_upd f s1 (S.slice s2 1 (S.length s2)) i (i + 1)
+        (f (S.head (S.slice s1 i l)) (S.head s2))
     }
       S.slice
-        (Spec.QUIC.pointwise_op U8.logxor
-          (S.upd s1 i (U8.logxor (S.head (S.slice s1 i l)) (S.head s2)))
+        (Spec.QUIC.pointwise_op f
+          (S.upd s1 i (f (S.head (S.slice s1 i l)) (S.head s2)))
           (S.slice s2 1 (S.length s2))
           (i + 1))
         i l;
@@ -467,19 +444,35 @@ let rec lemma_xor_inplace0 (s1 s2: S.seq U8.t) (i: nat): Lemma
     ()
 #pop-options
 
-let lemma_xor_inplace (s1 s2: S.seq U8.t): Lemma
-  (requires (S.length s1 = S.length s2))
-  (ensures (
-    let l = S.length s1 in
-    Spec.Loops.seq_map2 U8.logxor s1 s2 `S.equal`
-    Spec.QUIC.xor_inplace s1 s2 0))
-=
-  lemma_xor_inplace0 s1 s2 0
+val xor_inplace (dst src: B.buffer U8.t) (len: U32.t { B.length dst = U32.v len }):
+  Stack unit
+    (requires fun h0 ->
+      B.(all_live h0 [ buf dst; buf src ]) /\
+      B.disjoint dst src /\
+      B.length dst = B.length src)
+    (ensures fun h0 _ h1 ->
+      B.(modifies (loc_buffer dst) h0 h1) /\
+      B.as_seq h1 dst `S.equal` Spec.QUIC.xor_inplace (B.as_seq h0 dst) (B.as_seq h0 src) 0)
 
 let xor_inplace dst src len =
   let h0 = ST.get () in
   C.Loops.in_place_map2 dst src len U8.logxor;
-  lemma_xor_inplace (B.as_seq h0 dst) (B.as_seq h0 src)
+  pointwise_seq_map2 U8.logxor (B.as_seq h0 dst) (B.as_seq h0 src) 0
+
+val and_inplace (dst src: B.buffer U8.t) (len: U32.t { B.length dst = U32.v len }):
+  Stack unit
+    (requires fun h0 ->
+      B.(all_live h0 [ buf dst; buf src ]) /\
+      B.disjoint dst src /\
+      B.length dst = B.length src)
+    (ensures fun h0 _ h1 ->
+      B.(modifies (loc_buffer dst) h0 h1) /\
+      B.as_seq h1 dst `S.equal` Spec.QUIC.and_inplace (B.as_seq h0 dst) (B.as_seq h0 src) 0)
+
+let and_inplace dst src len =
+  let h0 = ST.get () in
+  C.Loops.in_place_map2 dst src len U8.logand;
+  pointwise_seq_map2 U8.logand (B.as_seq h0 dst) (B.as_seq h0 src) 0
 
 let encrypt #i s dst h plain plain_len pn_len =
   let State hash_alg aead_alg e_traffic_secret e_initial_pn aead_state iv hp_key pn = !*s in
